src/x86/instrrules/not.v
@@ -6,6 +6,14 @@ Lemma NOT_rule d (src:RegMem d) v:
   |-- specAtRegMemDst src (fun V => basic (V v) (UOP d OP_NOT src) empOP (V (invB v))).
 Proof. do_instrrule_triple. Qed.
 
+(** We make this rule an instance of the typeclass, after unfolding various things in its type. *)
+Section handle_type_of_rule.
+  Context d (src : RegMem d).
+  Let rule := @NOT_rule d src.
+  Let T := Eval cbv beta iota zeta delta [specAtRegMemDst] in (fun T (x : T) => T) _ rule.
+  Global Instance: instrrule (UOP d OP_NOT src) := rule : T.
+End handle_type_of_rule.
+
 Ltac basicNOT :=
   rewrite /makeUOP;
   let R := lazymatch goal with
