src/x86/instrrules/out.v
@@ -7,3 +7,6 @@ Lemma OUT_I_rule (c: BYTE) d :
   |-- basic
       (BYTEregIs AL d) (OUT c, AL) (outOP (zeroExtend 8 c) d) (BYTEregIs AL d).
 Proof. instrrule_triple_bazooka. by triple.core.triple_by_compute. Qed.
+
+(** We make this rule an instance of the typeclass, after unfolding various things in its type. *)
+Instance: forall (c : BYTE), instrrule (OUT c, AL) := @OUT_I_rule.
