src/x86/instrrules/pop.v
@@ -9,6 +9,14 @@ Lemma POP_rule (rm:RegMem true) (sp:DWORD) (oldv v:DWORD):
             (V v    ** ESP ~= sp+#4 ** sp:->v)).
 Proof. do_instrrule_triple. Qed.
 
+(** We make this rule an instance of the typeclass, after unfolding various things in its type. *)
+Section handle_type_of_rule.
+  Context (rm : RegMem true).
+  Let rule := @POP_rule rm.
+  Let T := Eval cbv beta iota zeta delta [specAtRegMemDst] in (fun T (x : T) => T) _ rule.
+  Global Instance: instrrule (POP rm) := rule : T.
+End handle_type_of_rule.
+
 Ltac basicPOP :=
   let R := lazymatch goal with
              | |- |-- basic ?p (POP ?a) ?O ?q => constr:(POP_rule a)
