src/x86/instrrules/ret.v
@@ -23,3 +23,14 @@ Proof.
   apply: TRIPLE_safeLater => R.
   do_instrrule_triple.
 Qed.
+
+(** We make this rule an instance of the typeclass, after unfolding various things in its type. *)
+Section handle_type_of_rule.
+  Context (offset : WORD).
+  Let rule := (fun p' sp => @RET_rule p' sp offset).
+  Let loopy_rule := (fun p' sp => @RET_loopy_rule p' sp offset).
+  Let T := Eval cbv beta iota zeta in (fun T (x : T) => T) _ rule.
+  Let loopy_T := Eval cbv beta iota zeta in (fun T (x : T) => T) _ loopy_rule.
+  Global Instance: instrrule (RETOP offset) := rule : T.
+  Global Instance: instrrule_loopy (RETOP offset) := loopy_rule : loopy_T.
+End handle_type_of_rule.
