src/x86/instrrules/shift.v
@@ -10,7 +10,7 @@ Proof. do 32 case => //.
 Qed.
 
 Lemma SHL_RI_rule (r:Reg) (v:DWORD) (count:nat):
-  count < 32 ->
+  count < n32 ->
   |-- basic (r~=v ** OSZCP?) (SHL r, count) empOP
             (r~=iter count shlB v ** OSZCP?).
 Proof.
@@ -26,7 +26,7 @@ Proof.
 Qed.
 
 Lemma SHR_RI_rule (r:Reg) (v:DWORD) (count:nat):
-  count < 32 ->
+  count < n32 ->
   |-- basic (r~=v ** OSZCP?) (SHR r, count) empOP
             (r~=iter count shrB v ** OSZCP?).
 Proof.
@@ -40,3 +40,7 @@ Proof.
             | progress rewrite /stateIsAny ]
        | destruct count as [|count]; rewrite /(iter 0) ?droplsb_iter_shrB ].
 Qed.
+
+(** We make this rule an instance of the typeclass, after unfolding various things in its type. *)
+Global Instance: forall (r : Reg) (count : nat), instrrule (SHL r, count) := fun r count v => @SHL_RI_rule r v count.
+Global Instance: forall (r : Reg) (count : nat), instrrule (SHR r, count) := fun r count v => @SHR_RI_rule r v count.
